Wrap up literal for now

ulib/FStar.List.Tot.Base.fst
@@ -556,3 +556,13 @@ let rec list_unref #a #p l =
     match l with
     | [] -> []
     | x::xs -> x :: list_unref xs
+
+val list_ref: #a:eqtype -> #p:(a -> bool) ->
+  l:list a { for_all p l } ->
+  l':list (x:a{ p x }) {
+    length l = length l' /\
+    (forall i. {:pattern (index l i) } index l i = index l' i) }
+let rec list_ref #a #p l =
+  match l with
+  | hd :: tl -> hd :: list_ref #a #p tl
+  | [] -> []
