ulib/LowStar.Literal.fst
@@ -1,0 +1,29 @@
+module LowStar.Literal
+
+module B = LowStar.Buffer
+module MB = LowStar.Monotonic.Buffer
+module IB = LowStar.ImmutableBuffer
+module HS = FStar.HyperStack
+module ST = FStar.HyperStack.ST
+
+open FStar.Mul
+
+/// The implementation of LowStar.Literal.fsti. Not extracted as-is but instead
+/// implemented in C using native string literals.
+
+let buffer_of_literal s =
+  let init: list UInt8.t = List.Tot.map u8_of_ascii_char (ascii_chars_of_ascii_string s) in
+  normalize_spec (List.Tot.length init <= UInt.max_int 32);
+  let h0 = ST.get () in
+  let b = IB.igcmalloc_of_list HS.root init in
+  let h1 = ST.get () in
+  // Note: our memory model isn't fine-grained enough to account for things
+  // allocated in the data-segment at program load-time and which remains always
+  // live. However, we wish for this function to remain in the Stack and expose
+  // no allocation behavior to its client. So, we cheat a little bit here.
+  assume (ST.equal_domains h0 h1);
+  b
+
+let const_string = s:string { zero_free s }
+
+let const_string_of_literal s = s
